


|样本|x1|x2|y|
|--|--|--|--|
|1|1|1|3.2|
|2|2|3|4.1|
|3|3|4|4.8|
|4|4|3|5.1|

$$
J = \sum_{i=1}^n [y_i - (a_1 x_{i,1} + a_2 x_{i,2}+b)]^2 \tag{2.2.1}
$$

$$
y_1 = a_1 x_{1,1}+a_2 x_{1,2} + b
\\\\
y_2 = a_1 x_{2,1}+a_2 x_{2,2} + b
\\\\
y_3 = a_1 x_{3,1}+a_2 x_{3,2} + b
\\\\
y_4 = a_1 x_{4,1}+a_2 x_{4,2} + b
\tag{2.2.2}
$$

$$
3.2=1·a_1+1·a_2+b
\\\\
4.1=2·a_1+3·a_2+b
\\\\
4.8=3·a_1+4·a_2+b
\\\\
5.1=4·a_1+3·a_2+b
$$

$$
\begin{aligned}
J &= \sum_{i=1}^n (y_i - \hat{y}_i)^2 = \sum_{i=1}^n error_i^2
\\\\
&=[3.2-(\hat{a}_1+\hat{a}_2+b)]^2
\\\\
&+[4.1-(2\hat{a}_1+3\hat{a}_2+\hat{b})]^2
\\\\
&+[4.8-(3\hat{a}_1+4\hat{a}_2+\hat{b})]^2
\\\\
&+[5.1-(4\hat{a}_1+3\hat{a}_2+\hat{b})]^2
\end{aligned}
\tag{1.3.1}
$$

$$
\begin{cases}
\frac{\partial J}{\partial \hat{a}_1} = -2(3.2-\hat{a}_1-\hat{a}_2-\hat{b})-4(4.1-2\hat{a}_1-3\hat{a}_2-\hat{b})-6(4.8-3\hat{a}_1-4\hat{a}_2-\hat{b})-8(5.1-4\hat{a}_1-3\hat{a}_2-\hat{b})=0
\\\\
\frac{\partial J}{\partial \hat{a}_2} = -2(3.2-\hat{a}_1-\hat{a}_2-\hat{b})-6(4.1-2\hat{a}_1-3\hat{a}_2-\hat{b})-8(4.8-3\hat{a}_1-4\hat{a}_2-\hat{b})-6(5.1-4\hat{a}_1-3\hat{a}_2-\hat{b})=0
\\\\
\frac{\partial J}{\partial \hat{b}} = -2(3.2-\hat{a}_1-\hat{a}_2-\hat{b})-2(4.1-2\hat{a}_1-3\hat{a}_2-\hat{b})-2(4.8-3\hat{a}_1-4\hat{a}_2-\hat{b})-2(5.1-4\hat{a}_1-3\hat{a}_2-\hat{b})=0
\end{cases}
$$

$$
\begin{cases}
60\hat{a}_1+62\hat{a}_2+20\hat{b}=92.4
\\\\
62\hat{a}_1+70\hat{a}_2+22\hat{b}=100
\\\\
20\hat{a}_1+22\hat{a}_2+8\hat{b}=34.4
\end{cases}
$$

$$
\begin{cases}

b=2.5
\\\\
\hat{a}_1=0.5
\\\\
\hat{a}_2=0.2
\end{cases}
$$

